chore: prepare for cleaning up `String` namespace

src/Init/Data/String/Basic.lean
@@ -58,6 +58,14 @@ theorem ByteArray.IsValidUTF8.append {b b' : ByteArray} (h : IsValidUTF8 b) (h' 
   rcases h' with ⟨m', rfl⟩
   exact .intro (m ++ m') (by simp)
 
+@[simp]
+theorem Char.toUInt8_val {c : Char} : c.val.toUInt8 = c.toUInt8 := rfl
+
+theorem ByteArray.IsValidUTF8.push {b : ByteArray} (h : IsValidUTF8 b) {c : Char} (hc : c.utf8Size = 1) :
+    IsValidUTF8 (b.push c.toUInt8) := by
+  rcases h with ⟨m, rfl⟩
+  refine ⟨m ++ [c], by simp [List.utf8Encode_singleton, String.utf8EncodeChar_eq_singleton hc]⟩
+
 theorem ByteArray.isValidUTF8_utf8Encode_singleton_append_iff {b : ByteArray} {c : Char} :
     IsValidUTF8 ([c].utf8Encode ++ b) ↔ IsValidUTF8 b := by
   refine ⟨?_, fun h => IsValidUTF8.append isValidUTF8_utf8Encode h⟩
@@ -1703,6 +1711,10 @@ Returns the byte at the position `pos` of a string.
 def ValidPos.byte {s : String} (pos : s.ValidPos) (h : pos ≠ s.endValidPos) : UInt8 :=
   pos.toSlice.byte (ne_of_apply_ne Slice.Pos.ofSlice (by simp [h]))
 
+theorem ValidPos.isUTF8FirstByte_byte {s : String} {pos : s.ValidPos} {h : pos ≠ s.endValidPos} :
+    (pos.byte h).IsUTF8FirstByte :=
+  Slice.Pos.isUTF8FirstByte_byte
+
 @[simp]
 theorem append_left_inj {s₁ s₂ : String} (t : String) :
     s₁ ++ t = s₂ ++ t ↔ s₁ = s₂ := by
@@ -1903,6 +1915,10 @@ theorem Slice.Pos.utf8ByteSize_byte {s : Slice} {pos : s.Pos} {h : pos ≠ s.end
     (pos.byte h).utf8ByteSize pos.isUTF8FirstByte_byte = (pos.get h).utf8Size := by
   simp [getUTF8Byte, byte, String.getUTF8Byte, get_eq_utf8DecodeChar, ByteArray.utf8Size_utf8DecodeChar]
 
+theorem ValidPos.utf8ByteSize_byte {s : String} {pos : s.ValidPos} {h : pos ≠ s.endValidPos} :
+    (pos.byte h).utf8ByteSize pos.isUTF8FirstByte_byte = (pos.get h).utf8Size :=
+  Slice.Pos.utf8ByteSize_byte
+
 /--
 Advances `p` by `n` bytes. This is not an `HAdd` instance because it should be a relatively
 rare operation, so we use a name to make accidental use less likely. To add the size of a
@@ -1968,9 +1984,14 @@ def Slice.Pos.next! {s : Slice} (pos : s.Pos) : s.Pos :=
   if h : pos = s.endPos then panic! "Cannot advance the end position" else pos.next h
 
 @[simp]
+theorem Slice.Pos.offset_next {s : Slice} {pos : s.Pos} {h : pos ≠ s.endPos} :
+    (pos.next h).offset = pos.offset + pos.get h := by
+  ext
+  simp [next, utf8ByteSize_byte]
+
 theorem Slice.Pos.byteIdx_offset_next {s : Slice} {pos : s.Pos} {h : pos ≠ s.endPos} :
     (pos.next h).offset.byteIdx = pos.offset.byteIdx + (pos.get h).utf8Size := by
-  simp [next, utf8ByteSize_byte]
+  simp
 
 @[simp]
 theorem Slice.Pos.lt_next {s : Slice} {pos : s.Pos} {h : pos ≠ s.endPos} :
@@ -2259,16 +2280,23 @@ def Slice.Pos.prevn {s : Slice} (p : s.Pos) (n : Nat) : s.Pos :=
       p
 
 @[expose]
-def utf8GetAux : List Char → Pos.Raw → Pos.Raw → Char
+def Pos.Raw.utf8GetAux : List Char → Pos.Raw → Pos.Raw → Char
   | [],    _, _ => default
   | c::cs, i, p => if i = p then c else utf8GetAux cs (i + c) p
+
+@[deprecated Pos.Raw.utf8GetAux (since := "2025-10-09")]
+abbrev utf8GetAux : List Char → Pos.Raw → Pos.Raw → Char :=
+  Pos.Raw.utf8GetAux
 
 /--
 Returns the character at position `p` of a string. If `p` is not a valid position, returns the
 fallback value `(default : Char)`, which is `'A'`, but does not panic.
 
 This function is overridden with an efficient implementation in runtime code. See
-`String.utf8GetAux` for the reference implementation.
+`String.Pos.Raw.utf8GetAux` for the reference implementation.
+
+This is a legacy function. The recommended alternative is `String.ValidPos.get`, combined with
+`String.pos` or another means of obtaining a `String.ValidPos`.
 
 Examples:
 * `"abc".get ⟨1⟩ = 'b'`
@@ -2279,32 +2307,27 @@ Examples:
 def Pos.Raw.get (s : @& String) (p : @& Pos.Raw) : Char :=
   utf8GetAux s.data 0 p
 
-/--
-Returns the character at position `p` of a string. If `p` is not a valid position, returns the
-fallback value `(default : Char)`, which is `'A'`, but does not panic.
-
-This function is overridden with an efficient implementation in runtime code. See
-`String.utf8GetAux` for the reference implementation.
-
-Examples:
-* `"abc".get ⟨1⟩ = 'b'`
-* `"abc".get ⟨3⟩ = (default : Char)` because byte `3` is at the end of the string.
-* `"L∃∀N".get ⟨2⟩ = (default : Char)` because byte `2` is in the middle of `'∃'`.
--/
-@[extern "lean_string_utf8_get", expose]
+@[extern "lean_string_utf8_get", expose, inherit_doc Pos.Raw.get]
 def get (s : @& String) (p : @& Pos.Raw) : Char :=
-  utf8GetAux s.data 0 p
+  Pos.Raw.utf8GetAux s.data 0 p
 
 @[expose]
-def utf8GetAux? : List Char → Pos.Raw → Pos.Raw → Option Char
+def Pos.Raw.utf8GetAux? : List Char → Pos.Raw → Pos.Raw → Option Char
   | [],    _, _ => none
   | c::cs, i, p => if i = p then some c else utf8GetAux? cs (i + c) p
+
+@[deprecated Pos.Raw.utf8GetAux (since := "2025-10-09")]
+abbrev utf8GetAux? : List Char → Pos.Raw → Pos.Raw → Option Char :=
+  Pos.Raw.utf8GetAux?
 
 /--
 Returns the character at position `p` of a string. If `p` is not a valid position, returns `none`.
 
 This function is overridden with an efficient implementation in runtime code. See
 `String.utf8GetAux?` for the reference implementation.
+
+This is a legacy function. The recommended alternative is `String.ValidPos.get`, combined with
+`String.pos?` or another means of obtaining a `String.ValidPos`.
 
 Examples:
 * `"abc".get? ⟨1⟩ = some 'b'`
@@ -2316,29 +2339,20 @@ Examples:
 def Pos.Raw.get? : (@& String) → (@& Pos.Raw) → Option Char
   | s, p => utf8GetAux? s.data 0 p
 
-/--
-Returns the character at position `p` of a string. If `p` is not a valid position, returns `none`.
-
-This function is overridden with an efficient implementation in runtime code. See
-`String.utf8GetAux?` for the reference implementation.
-
-Examples:
-* `"abc".get? ⟨1⟩ = some 'b'`
-* `"abc".get? ⟨3⟩ = none`
-* `"L∃∀N".get? ⟨1⟩ = some '∃'`
-* `"L∃∀N".get? ⟨2⟩ = none`
--/
-@[extern "lean_string_utf8_get_opt", expose]
+@[extern "lean_string_utf8_get_opt", expose, inherit_doc Pos.Raw.get?]
 def get? : (@& String) → (@& Pos.Raw) → Option Char
-  | s, p => utf8GetAux? s.data 0 p
+  | s, p => Pos.Raw.utf8GetAux? s.data 0 p
 
 /--
 Returns the character at position `p` of a string. Panics if `p` is not a valid position.
 
-See `String.get?` for a safer alternative.
+See `String.pos?` and `String.ValidPos.get` for a safer alternative.
 
 This function is overridden with an efficient implementation in runtime code. See
 `String.utf8GetAux` for the reference implementation.
+
+This is a legacy function. The recommended alternative is `String.ValidPos.get`, combined with
+`String.pos!` or another means of obtaining a `String.ValidPos`.
 
 Examples
 * `"abc".get! ⟨1⟩ = 'b'`
@@ -2346,29 +2360,171 @@ Examples
 @[extern "lean_string_utf8_get_bang", expose]
 def Pos.Raw.get! (s : @& String) (p : @& Pos.Raw) : Char :=
   match s with
-  | s => utf8GetAux s.data 0 p
+  | s => Pos.Raw.utf8GetAux s.data 0 p
 
-/--
-Returns the character at position `p` of a string. Panics if `p` is not a valid position.
-
-See `String.get?` for a safer alternative.
-
-This function is overridden with an efficient implementation in runtime code. See
-`String.utf8GetAux` for the reference implementation.
-
-Examples
-* `"abc".get! ⟨1⟩ = 'b'`
--/
-@[extern "lean_string_utf8_get_bang", expose]
+@[extern "lean_string_utf8_get_bang", expose, inherit_doc Pos.Raw.get!]
 def get! (s : @& String) (p : @& Pos.Raw) : Char :=
   match s with
-  | s => utf8GetAux s.data 0 p
+  | s => Pos.Raw.utf8GetAux s.data 0 p
 
 @[expose]
-def utf8SetAux (c' : Char) : List Char → Pos.Raw → Pos.Raw → List Char
+def Pos.Raw.utf8SetAux (c' : Char) : List Char → Pos.Raw → Pos.Raw → List Char
   | [],    _, _ => []
   | c::cs, i, p =>
     if i = p then (c'::cs) else c::(utf8SetAux c' cs (i + c) p)
+
+@[deprecated Pos.Raw.utf8SetAux (since := "2025-10-09")]
+abbrev utf8SetAux (c' : Char) : List Char → Pos.Raw → Pos.Raw → List Char :=
+  Pos.Raw.utf8SetAux c'
+
+@[simp]
+theorem ValidPos.toSlice_get {s : String} {p : s.ValidPos} {h} :
+    p.toSlice.get h = p.get (ne_of_apply_ne (·.toSlice) (by simp_all)) := by
+  rfl
+
+@[simp]
+theorem ValidPos.offset_next {s : String} (p : s.ValidPos) (h : p ≠ s.endValidPos) :
+    (p.next h).offset = p.offset + p.get h := by
+  simp [next]
+
+theorem ValidPos.byteIdx_offset_next {s : String} (p : s.ValidPos) (h : p ≠ s.endValidPos) :
+    (p.next h).offset.byteIdx = p.offset.byteIdx + (p.get h).utf8Size := by
+  simp
+
+theorem ValidPos.byteIdx_lt_utf8ByteSize {s : String} (p : s.ValidPos) (h : p ≠ s.endValidPos) :
+    p.offset.byteIdx < s.utf8ByteSize := by
+  have := byteIdx_endPos ▸ Pos.Raw.le_iff.1 p.isValid.le_endPos
+  simp only [ne_eq, ValidPos.ext_iff, offset_endValidPos, Pos.Raw.ext_iff, byteIdx_endPos] at h
+  omega
+
+@[simp]
+theorem ValidPos.str_toSlice {s : String} {p : s.ValidPos} : p.toSlice.str = p := by
+  ext
+  simp
+
+/-- The slice from the beginning of `s` up to `p` (exclusive). -/
+@[inline, expose]
+def replaceEnd (s : String) (p : s.ValidPos) : Slice :=
+  s.toSlice.replaceEnd p.toSlice
+
+@[simp]
+theorem str_replaceEnd {s : String} {p : s.ValidPos} : (s.replaceEnd p).str = s := rfl
+
+@[simp]
+theorem startInclusive_replaceEnd {s : String} {p : s.ValidPos} :
+    (s.replaceEnd p).startInclusive = s.startValidPos := by
+  simp [replaceEnd]
+
+@[simp]
+theorem endExclusive_replaceEnd {s : String} {p : s.ValidPos} :
+    (s.replaceEnd p).endExclusive = p := by
+  simp [replaceEnd]
+
+theorem Pos.Raw.isValidForSlice_stringReplaceEnd {s : String} {p : s.ValidPos} {q : Pos.Raw} :
+    q.IsValidForSlice (s.replaceEnd p) ↔ q ≤ p.offset ∧ q.IsValid s := by
+  rw [replaceEnd, isValidForSlice_replaceEnd, ValidPos.offset_toSlice, isValidForSlice_toSlice_iff]
+
+/-- The slice from `p` (inclusive) up to the end of `s`. -/
+@[inline, expose]
+def replaceStart (s : String) (p : s.ValidPos) : Slice :=
+  s.toSlice.replaceStart p.toSlice
+
+@[simp]
+theorem str_replaceStart {s : String} {p : s.ValidPos} : (s.replaceStart p).str = s := rfl
+
+@[simp]
+theorem startInclusive_replaceStart {s : String} {p : s.ValidPos} :
+    (s.replaceStart p).startInclusive = p := by
+  simp [replaceStart]
+
+@[simp]
+theorem endExclusive_replaceStart {s : String} {p : s.ValidPos} :
+    (s.replaceStart p).endExclusive = s.endValidPos := by
+  simp [replaceStart]
+
+theorem Pos.Raw.isValidForSlice_stringReplaceStart {s : String} {p : s.ValidPos} {q : Pos.Raw} :
+    q.IsValidForSlice (s.replaceStart p) ↔ (q.offsetBy p.offset).IsValid s := by
+  rw [replaceStart, isValidForSlice_replaceStart, isValidForSlice_toSlice_iff,
+    ValidPos.offset_toSlice]
+
+/--
+Replaces the character at a specified position in a string with a new character.
+
+If both the replacement character and the replaced character are 7-bit ASCII characters and the
+string is not shared, then it is updated in-place and not copied.
+
+Examples:
+* `("abc".pos ⟨1⟩ (by decide)).set 'B' (by decide) = "aBc"`
+* `("L∃∀N".pos ⟨4⟩ (by decide)).set 'X' (by decide) = "L∃XN"`
+-/
+@[extern "lean_string_utf8_set", expose]
+def ValidPos.set {s : String} (p : s.ValidPos) (c : Char) (hp : p ≠ s.endValidPos) : String :=
+  if hc : c.utf8Size = 1 ∧ (p.byte hp).utf8ByteSize isUTF8FirstByte_byte = 1 then
+    .ofByteArray (s.bytes.set p.offset.byteIdx c.toUInt8 (p.byteIdx_lt_utf8ByteSize hp)) (by
+      rw [ByteArray.set_eq_push_extract_append_extract, ← hc.2, utf8ByteSize_byte,
+        ← ValidPos.byteIdx_offset_next]
+      refine ByteArray.IsValidUTF8.append ?_ (p.next hp).isValid.isValidUTF8_extract_utf8ByteSize
+      exact p.isValid.isValidUTF8_extract_zero.push hc.1)
+  else
+    (s.replaceEnd p).copy ++ singleton c ++ (s.replaceStart (p.next hp)).copy
+
+theorem ValidPos.set_eq_append {s : String} {p : s.ValidPos} {c : Char} {hp} :
+    p.set c hp = (s.replaceEnd p).copy ++ singleton c ++ (s.replaceStart (p.next hp)).copy := by
+  rw [set]
+  split
+  · rename_i h
+    simp [← bytes_inj, ByteArray.set_eq_push_extract_append_extract, Slice.bytes_copy,
+      List.utf8Encode_singleton, String.utf8EncodeChar_eq_singleton h.1, utf8ByteSize_byte ▸ h.2]
+  · rfl
+
+theorem Pos.Raw.IsValid.set_of_le {s : String} {p : s.ValidPos} {c : Char} {hp : p ≠ s.endValidPos}
+    {q : Pos.Raw} (hq : q.IsValid s) (hpq : q ≤ p.offset) : q.IsValid (p.set c hp) := by
+  rw [ValidPos.set_eq_append, String.append_assoc]
+  apply append_right
+  rw [isValid_copy_iff, isValidForSlice_stringReplaceEnd]
+  exact ⟨hpq, hq⟩
+
+/-- Given a valid position in a string, obtain the corresponding position after setting a character on
+that string, provided that the position was before the changed position. -/
+@[inline]
+def ValidPos.setOfLE {s : String} (q p : s.ValidPos) (c : Char) (hp : p ≠ s.endValidPos)
+    (hpq : q ≤ p) : (p.set c hp).ValidPos where
+  offset := q.offset
+  isValid := q.isValid.set_of_le hpq
+
+@[simp]
+theorem ValidPos.offset_setOfLE {s : String} {q p : s.ValidPos} {c : Char} {hp : p ≠ s.endValidPos}
+    {hpq : q ≤ p} : (q.setOfLE p c hp hpq).offset = q.offset := (rfl)
+
+/--
+Replaces the character at position `p` in the string `s` with the result of applying `f` to that
+character.
+
+If both the replacement character and the replaced character are 7-bit ASCII characters and the
+string is not shared, then it is updated in-place and not copied.
+
+Examples:
+* `("abc".pos ⟨1⟩ (by decide)).modify Char.toUpper (by decide) = "aBc"`
+-/
+def ValidPos.modify {s : String} (p : s.ValidPos) (f : Char → Char) (hp : p ≠ s.endValidPos) :
+    String :=
+  p.set (f <| p.get hp) hp
+
+theorem Pos.Raw.IsValid.modify_of_le {s : String} {p : s.ValidPos} {f : Char → Char}
+    {hp : p ≠ s.endValidPos} {q : Pos.Raw} (hq : q.IsValid s) (hpq : q ≤ p.offset) :
+    q.IsValid (p.modify f hp) :=
+  set_of_le hq hpq
+
+/-- Given a valid position in a string, obtain the corresponding position after modifying a character
+in that string, provided that the position was before the changed position. -/
+def ValidPos.modifyOfLE {s : String} (q p : s.ValidPos) (f : Char → Char)
+    (hp : p ≠ s.endValidPos) (hpq : q ≤ p) : (p.modify f hp).ValidPos where
+  offset := q.offset
+  isValid := q.isValid.modify_of_le hpq
+
+@[simp]
+theorem ValidPos.offset_modifyOfLE {s : String} {q p : s.ValidPos} {f : Char → Char}
+    {hp : p ≠ s.endValidPos} {hpq : q ≤ p} : (q.modifyOfLE p f hp hpq).offset = q.offset := (rfl)
 
 /--
 Replaces the character at a specified position in a string with a new character. If the position is
@@ -2376,6 +2532,9 @@ invalid, the string is returned unchanged.
 
 If both the replacement character and the replaced character are 7-bit ASCII characters and the
 string is not shared, then it is updated in-place and not copied.
+
+This is a legacy function. The recommended alternative is `String.ValidPos.set`, combined with
+`String.pos` or another means of obtaining a `String.ValidPos`.
 
 Examples:
 * `"abc".set ⟨1⟩ 'B' = "aBc"`
@@ -2386,25 +2545,11 @@ Examples:
 -/
 @[extern "lean_string_utf8_set", expose]
 def Pos.Raw.set : String → (@& Pos.Raw) → Char → String
-  | s, i, c => (utf8SetAux c s.data 0 i).asString
+  | s, i, c => (Pos.Raw.utf8SetAux c s.data 0 i).asString
 
-/--
-Replaces the character at a specified position in a string with a new character. If the position is
-invalid, the string is returned unchanged.
-
-If both the replacement character and the replaced character are 7-bit ASCII characters and the
-string is not shared, then it is updated in-place and not copied.
-
-Examples:
-* `"abc".set ⟨1⟩ 'B' = "aBc"`
-* `"abc".set ⟨3⟩ 'D' = "abc"`
-* `"L∃∀N".set ⟨4⟩ 'X' = "L∃XN"`
-* `"L∃∀N".set ⟨2⟩ 'X' = "L∃∀N"` because `'∃'` is a multi-byte character, so the byte index `2` is an
-  invalid position.
--/
-@[extern "lean_string_utf8_set", expose]
+@[extern "lean_string_utf8_set", expose, inherit_doc Pos.Raw.set]
 def set : String → (@& Pos.Raw) → Char → String
-  | s, i, c => (utf8SetAux c s.data 0 i).asString
+  | s, i, c => (Pos.Raw.utf8SetAux c s.data 0 i).asString
 
 /--
 Replaces the character at position `p` in the string `s` with the result of applying `f` to that
@@ -2413,13 +2558,20 @@ character. If `p` is an invalid position, the string is returned unchanged.
 If both the replacement character and the replaced character are 7-bit ASCII characters and the
 string is not shared, then it is updated in-place and not copied.
 
+This is a legacy function. The recommended alternative is `String.ValidPos.set`, combined with
+`String.pos` or another means of obtaining a `String.ValidPos`.
+
 Examples:
 * `"abc".modify ⟨1⟩ Char.toUpper = "aBc"`
 * `"abc".modify ⟨3⟩ Char.toUpper = "abc"`
 -/
 @[expose]
+def Pos.Raw.modify (s : String) (i : Pos.Raw) (f : Char → Char) : String :=
+  i.set s (f (i.get s))
+
+@[expose, inherit_doc Pos.Raw.modify, deprecated Pos.Raw.modify (since := "2025-10-10")]
 def modify (s : String) (i : Pos.Raw) (f : Char → Char) : String :=
-  s.set i <| f <| s.get i
+  i.set s (f (i.get s))
 
 /--
 Returns the next position in a string after position `p`. If `p` is not a valid position or
@@ -2427,6 +2579,10 @@ Returns the next position in a string after position `p`. If `p` is not a valid 
 
 A run-time bounds check is performed to determine whether `p` is at the end of the string. If a
 bounds check has already been performed, use `String.next'` to avoid a repeated check.
+
+This is a legacy function. The recommended alternative is `String.ValidPos.next` or one of its
+variants like `String.ValidPos.next?`, combined with `String.pos` or another means of obtaining
+a `String.ValisPos`.
 
 Some examples of edge cases:
 * `"abc".next ⟨3⟩ = ⟨4⟩`, since `3 = "abc".endPos`
@@ -2441,32 +2597,21 @@ def Pos.Raw.next (s : @& String) (p : @& Pos.Raw) : Pos.Raw :=
   let c := get s p
   p + c
 
-/--
-Returns the next position in a string after position `p`. If `p` is not a valid position or
-`p = s.endPos`, returns the position one byte after `p`.
-
-A run-time bounds check is performed to determine whether `p` is at the end of the string. If a
-bounds check has already been performed, use `String.next'` to avoid a repeated check.
-
-Some examples of edge cases:
-* `"abc".next ⟨3⟩ = ⟨4⟩`, since `3 = "abc".endPos`
-* `"L∃∀N".next ⟨2⟩ = ⟨3⟩`, since `2` points into the middle of a multi-byte UTF-8 character
-
-Examples:
-* `"abc".get ("abc".next 0) = 'b'`
-* `"L∃∀N".get (0 |> "L∃∀N".next |> "L∃∀N".next) = '∀'`
--/
-@[extern "lean_string_utf8_next", expose]
+@[extern "lean_string_utf8_next", expose, inherit_doc Pos.Raw.next]
 def next (s : @& String) (p : @& Pos.Raw) : Pos.Raw :=
   let c := get s p
   p + c
 
 @[expose]
-def utf8PrevAux : List Char → Pos.Raw → Pos.Raw → Pos.Raw
+def Pos.Raw.utf8PrevAux : List Char → Pos.Raw → Pos.Raw → Pos.Raw
   | [],    _, p => ⟨p.byteIdx - 1⟩
   | c::cs, i, p =>
     let i' := i + c
     if p ≤ i' then i else utf8PrevAux cs i' p
+
+@[deprecated Pos.Raw.utf8PrevAux (since := "2025-10-10")]
+abbrev utf8PrevAux : List Char → Pos.Raw → Pos.Raw → Pos.Raw :=
+  Pos.Raw.utf8PrevAux
 
 /--
 Returns the position in a string before a specified position, `p`. If `p = ⟨0⟩`, returns `0`. If `p`
@@ -2475,6 +2620,10 @@ middle of a multi-byte character, returns the beginning position of that charact
 
 For example, `"L∃∀N".prev ⟨3⟩` is `⟨1⟩`, since byte 3 occurs in the middle of the multi-byte
 character `'∃'` that starts at byte 1.
+
+This is a legacy function. The recommended alternative is `String.ValidPos.prev` or one of its
+variants like `String.ValidPos.prev?`, combined with `String.pos` or another means of obtaining
+a `String.ValidPos`.
 
 Examples:
 * `"abc".get ("abc".endPos |> "abc".prev) = 'c'`
@@ -2484,21 +2633,9 @@ Examples:
 def Pos.Raw.prev : (@& String) → (@& Pos.Raw) → Pos.Raw
   | s, p => utf8PrevAux s.data 0 p
 
-/--
-Returns the position in a string before a specified position, `p`. If `p = ⟨0⟩`, returns `0`. If `p`
-is greater than `endPos`, returns the position one byte before `p`. Otherwise, if `p` occurs in the
-middle of a multi-byte character, returns the beginning position of that character.
-
-For example, `"L∃∀N".prev ⟨3⟩` is `⟨1⟩`, since byte 3 occurs in the middle of the multi-byte
-character `'∃'` that starts at byte 1.
-
-Examples:
-* `"abc".get ("abc".endPos |> "abc".prev) = 'c'`
-* `"L∃∀N".get ("L∃∀N".endPos |> "L∃∀N".prev |> "L∃∀N".prev |> "L∃∀N".prev) = '∃'`
--/
 @[extern "lean_string_utf8_prev", expose]
 def prev : (@& String) → (@& Pos.Raw) → Pos.Raw
-  | s, p => utf8PrevAux s.data 0 p
+  | s, p => Pos.Raw.utf8PrevAux s.data 0 p
 
 /--
 Returns the first character in `s`. If `s = ""`, returns `(default : Char)`.
@@ -2541,20 +2678,7 @@ Examples:
 def Pos.Raw.atEnd : (@& String) → (@& Pos.Raw) → Bool
   | s, p => p.byteIdx ≥ utf8ByteSize s
 
-/--
-Returns `true` if a specified byte position is greater than or equal to the position which points to
-the end of a string. Otherwise, returns `false`.
-
-Examples:
-* `(0 |> "abc".next |> "abc".next |> "abc".atEnd) = false`
-* `(0 |> "abc".next |> "abc".next |> "abc".next |> "abc".next |> "abc".atEnd) = true`
-* `(0 |> "L∃∀N".next |> "L∃∀N".next |> "L∃∀N".next |> "L∃∀N".atEnd) = false`
-* `(0 |> "L∃∀N".next |> "L∃∀N".next |> "L∃∀N".next |> "L∃∀N".next |> "L∃∀N".atEnd) = true`
-* `"abc".atEnd ⟨4⟩ = true`
-* `"L∃∀N".atEnd ⟨7⟩ = false`
-* `"L∃∀N".atEnd ⟨8⟩ = true`
--/
-@[extern "lean_string_utf8_at_end", expose]
+@[extern "lean_string_utf8_at_end", expose, inherit_doc Pos.Raw.atEnd]
 def atEnd : (@& String) → (@& Pos.Raw) → Bool
   | s, p => p.byteIdx ≥ utf8ByteSize s
 
@@ -2574,6 +2698,9 @@ def getInBounds? (s : String) (p : String.Pos) : Option Char :=
 Even with evidence of `¬ s.atEnd p`, `p` may be invalid if a byte index points into the middle of a
 multi-byte UTF-8 character. For example, `"L∃∀N".get' ⟨2⟩ (by decide) = (default : Char)`.
 
+This is a legacy function. The recommended alternative is `String.ValidPos.get`, combined with
+`String.pos` or another means of obtaining a `String.ValidPos`.
+
 Examples:
 * `"abc".get' 0 (by decide) = 'a'`
 * `let lean := "L∃∀N"; lean.get' (0 |> lean.next |> lean.next) (by decide) = '∀'`
@@ -2581,32 +2708,12 @@ Examples:
 @[extern "lean_string_utf8_get_fast", expose]
 def Pos.Raw.get' (s : @& String) (p : @& Pos.Raw) (h : ¬ s.atEnd p) : Char :=
   match s with
-  | s => utf8GetAux s.data 0 p
+  | s => Pos.Raw.utf8GetAux s.data 0 p
 
-/--
-Returns the character at position `p` of a string. Returns `(default : Char)`, which is `'A'`, if
-`p` is not a valid position.
-
-Requires evidence, `h`, that `p` is within bounds instead of performing a run-time bounds check as
-in `String.get`.
-
-A typical pattern combines `get'` with a dependent `if`-expression to avoid the overhead of an
-additional bounds check. For example:
-```
-def getInBounds? (s : String) (p : String.Pos) : Option Char :=
-  if h : s.atEnd p then none else some (s.get' p h)
-```
-Even with evidence of `¬ s.atEnd p`, `p` may be invalid if a byte index points into the middle of a
-multi-byte UTF-8 character. For example, `"L∃∀N".get' ⟨2⟩ (by decide) = (default : Char)`.
-
-Examples:
-* `"abc".get' 0 (by decide) = 'a'`
-* `let lean := "L∃∀N"; lean.get' (0 |> lean.next |> lean.next) (by decide) = '∀'`
--/
-@[extern "lean_string_utf8_get_fast", expose]
+@[extern "lean_string_utf8_get_fast", expose, inherit_doc Pos.Raw.get']
 def get' (s : @& String) (p : @& Pos.Raw) (h : ¬ s.atEnd p) : Char :=
   match s with
-  | s => utf8GetAux s.data 0 p
+  | s => Pos.Raw.utf8GetAux s.data 0 p
 
 /--
 Returns the next position in a string after position `p`. The result is unspecified if `p` is not a
@@ -2621,6 +2728,9 @@ an additional bounds check. For example:
 def next? (s : String) (p : String.Pos) : Option Char :=
   if h : s.atEnd p then none else s.get (s.next' p h)
 ```
+
+This is a legacy function. The recommended alternative is `String.ValidPos.next`, combined with
+`String.pos` or another means of obtaining a `String.ValidPos`.
 
 Example:
 * `let abc := "abc"; abc.get (abc.next' 0 (by decide)) = 'b'`
@@ -2630,42 +2740,34 @@ def Pos.Raw.next' (s : @& String) (p : @& Pos.Raw) (h : ¬ s.atEnd p) : Pos.Raw 
   let c := get s p
   p + c
 
-/--
-Returns the next position in a string after position `p`. The result is unspecified if `p` is not a
-valid position.
-
-Requires evidence, `h`, that `p` is within bounds. No run-time bounds check is performed, as in
-`String.next`.
-
-A typical pattern combines `String.next'` with a dependent `if`-expression to avoid the overhead of
-an additional bounds check. For example:
-```
-def next? (s : String) (p : String.Pos) : Option Char :=
-  if h : s.atEnd p then none else s.get (s.next' p h)
-```
-
-Example:
-* `let abc := "abc"; abc.get (abc.next' 0 (by decide)) = 'b'`
--/
-@[extern "lean_string_utf8_next_fast", expose]
+@[extern "lean_string_utf8_next_fast", expose, inherit_doc Pos.Raw.next']
 def next' (s : @& String) (p : @& Pos.Raw) (h : ¬ s.atEnd p) : Pos.Raw :=
   let c := get s p
   p + c
 
-@[deprecated Char.utf8Size_pos (since := "2026-06-04")] abbrev one_le_csize := Char.utf8Size_pos
+@[deprecated Pos.Raw.lt_iff (since := "2025-10-10")]
+theorem pos_lt_eq (p₁ p₂ : Pos.Raw) : (p₁ < p₂) = (p₁.1 < p₂.1) :=
+  propext Pos.Raw.lt_iff
 
-@[simp] theorem pos_lt_eq (p₁ p₂ : Pos.Raw) : (p₁ < p₂) = (p₁.1 < p₂.1) := rfl
-
-@[simp] theorem pos_add_char (p : Pos.Raw) (c : Char) : (p + c).byteIdx = p.byteIdx + c.utf8Size := rfl
+@[deprecated Pos.Raw.byteIdx_add_char (since := "2025-10-10")]
+theorem pos_add_char (p : Pos.Raw) (c : Char) : (p + c).byteIdx = p.byteIdx + c.utf8Size :=
+  Pos.Raw.byteIdx_add_char
 
 protected theorem Pos.Raw.ne_zero_of_lt : {a b : Pos.Raw} → a < b → b ≠ 0
   | _, _, hlt, rfl => Nat.not_lt_zero _ hlt
 
-theorem lt_next (s : String) (i : Pos.Raw) : i.1 < (s.next i).1 :=
+theorem Pos.Raw.lt_next (s : String) (i : Pos.Raw) : i < i.next s :=
   Nat.add_lt_add_left (Char.utf8Size_pos _) _
 
-theorem utf8PrevAux_lt_of_pos : ∀ (cs : List Char) (i p : Pos.Raw), i < p → p ≠ 0 →
-    (utf8PrevAux cs i p).1 < p.1
+theorem Pos.Raw.byteIdx_lt_byteIdx_next (s : String) (i : Pos.Raw) : i.1 < (i.next s).1 :=
+  lt_iff.1 (i.lt_next s)
+
+@[deprecated Pos.Raw.byteIdx_lt_byteIdx_next (since := "2025-10-10")]
+theorem lt_next (s : String) (i : Pos.Raw) : i.1 < (s.next i).1 :=
+  Pos.Raw.lt_next s i
+
+theorem Pos.Raw.utf8PrevAux_lt_of_pos : ∀ (cs : List Char) (i p : Pos.Raw), i < p → p ≠ 0 →
+    (Pos.Raw.utf8PrevAux cs i p).1 < p.1
   | [], _, _, _, h => Nat.sub_one_lt (mt (congrArg Pos.Raw.mk) h)
   | c::cs, i, p, h, h' => by
     simp [utf8PrevAux]
@@ -2673,14 +2775,18 @@ theorem utf8PrevAux_lt_of_pos : ∀ (cs : List Char) (i p : Pos.Raw), i < p → 
     next => exact h
     next => exact utf8PrevAux_lt_of_pos _ _ _ (Nat.lt_of_not_le h'') h'
 
-theorem prev_lt_of_pos (s : String) (i : Pos.Raw) (h : i ≠ 0) : (s.prev i).1 < i.1 :=
+theorem Pos.Raw.prev_lt_of_pos (s : String) (i : Pos.Raw) (h : i ≠ 0) : (s.prev i).1 < i.1 :=
   utf8PrevAux_lt_of_pos _ _ _ (Nat.zero_lt_of_ne_zero (mt (congrArg Pos.Raw.mk) h)) h
+
+@[deprecated Pos.Raw.prev_lt_of_pos (since := "2025-10-10")]
+theorem prev_lt_of_pos (s : String) (i : Pos.Raw) (h : i ≠ 0) : (s.prev i).1 < i.1 :=
+  Pos.Raw.prev_lt_of_pos s i h
 
 def posOfAux (s : String) (c : Char) (stopPos : Pos.Raw) (pos : Pos.Raw) : Pos.Raw :=
   if h : pos < stopPos then
     if s.get pos == c then pos
     else
-      have := Nat.sub_lt_sub_left h (lt_next s pos)
+      have := Nat.sub_lt_sub_left h (Pos.Raw.lt_next s pos)
       posOfAux s c stopPos (s.next pos)
   else pos
 termination_by stopPos.1 - pos.1
@@ -2704,7 +2810,7 @@ def Internal.posOfImpl (s : String) (c : Char) : Pos.Raw :=
 def revPosOfAux (s : String) (c : Char) (pos : Pos.Raw) : Option Pos.Raw :=
   if h : pos = 0 then none
   else
-    have := prev_lt_of_pos s pos h
+    have := Pos.Raw.prev_lt_of_pos s pos h
     let pos := s.prev pos
     if s.get pos == c then some pos
     else revPosOfAux s c pos
@@ -2726,7 +2832,7 @@ def findAux (s : String) (p : Char → Bool) (stopPos : Pos.Raw) (pos : Pos.Raw)
   if h : pos < stopPos then
     if p (s.get pos) then pos
     else
-      have := Nat.sub_lt_sub_left h (lt_next s pos)
+      have := Nat.sub_lt_sub_left h (Pos.Raw.lt_next s pos)
       findAux s p stopPos (s.next pos)
   else pos
 termination_by stopPos.1 - pos.1
@@ -2747,7 +2853,7 @@ Examples:
 def revFindAux (s : String) (p : Char → Bool) (pos : Pos.Raw) : Option Pos.Raw :=
   if h : pos = 0 then none
   else
-    have := prev_lt_of_pos s pos h
+    have := Pos.Raw.prev_lt_of_pos s pos h
     let pos := s.prev pos
     if p (s.get pos) then some pos
     else revFindAux s p pos
@@ -2794,7 +2900,7 @@ def firstDiffPos (a b : String) : Pos.Raw :=
     if h : i < stopPos then
       if a.get i != b.get i then i
       else
-        have := Nat.sub_lt_sub_left h (lt_next a i)
+        have := Nat.sub_lt_sub_left h (Pos.Raw.lt_next a i)
         loop (a.next i)
     else i
     termination_by stopPos.1 - i.1
@@ -2806,6 +2912,10 @@ Creates a new string that consists of the region of the input string delimited b
 The result is `""` if the start position is greater than or equal to the end position or if the
 start position is at the end of the string. If either position is invalid (that is, if either points
 at the middle of a multi-byte UTF-8 character) then the result is unspecified.
+
+This is a legacy function. The recommended alternative is `String.ValidPos.extract`, but usually
+it is even better to operate on `String.Slice` instead and call `String.Slice.copy` (only) if
+required.
 
 Examples:
 * `"red green blue".extract ⟨0⟩ ⟨3⟩ = "red"`
@@ -2827,39 +2937,16 @@ where
     | [],    _, _ => []
     | c::cs, i, e => if i = e then [] else c :: go₂ cs (i + c) e
 
-/--
-Creates a new string that consists of the region of the input string delimited by the two positions.
-
-The result is `""` if the start position is greater than or equal to the end position or if the
-start position is at the end of the string. If either position is invalid (that is, if either points
-at the middle of a multi-byte UTF-8 character) then the result is unspecified.
-
-Examples:
-* `"red green blue".extract ⟨0⟩ ⟨3⟩ = "red"`
-* `"red green blue".extract ⟨3⟩ ⟨0⟩ = ""`
-* `"red green blue".extract ⟨0⟩ ⟨100⟩ = "red green blue"`
-* `"red green blue".extract ⟨4⟩ ⟨100⟩ = "green blue"`
-* `"L∃∀N".extract ⟨1⟩ ⟨2⟩ = "∃∀N"`
-* `"L∃∀N".extract ⟨2⟩ ⟨100⟩ = ""`
--/
 @[extern "lean_string_utf8_extract", expose]
 def extract : (@& String) → (@& Pos.Raw) → (@& Pos.Raw) → String
-  | s, b, e => if b.byteIdx ≥ e.byteIdx then "" else (go₁ s.data 0 b e).asString
-where
-  go₁ : List Char → Pos.Raw → Pos.Raw → Pos.Raw → List Char
-    | [],        _, _, _ => []
-    | s@(c::cs), i, b, e => if i = b then go₂ s i e else go₁ cs (i + c) b e
-
-  go₂ : List Char → Pos.Raw → Pos.Raw → List Char
-    | [],    _, _ => []
-    | c::cs, i, e => if i = e then [] else c :: go₂ cs (i + c) e
+  | s, b, e => Pos.Raw.extract s b e
 
 @[specialize] def splitAux (s : String) (p : Char → Bool) (b : Pos.Raw) (i : Pos.Raw) (r : List String) : List String :=
   if h : s.atEnd i then
     let r := (s.extract b i)::r
     r.reverse
   else
-    have := Nat.sub_lt_sub_left (Nat.gt_of_not_le (mt decide_eq_true h)) (lt_next s _)
+    have := Nat.sub_lt_sub_left (Nat.gt_of_not_le (mt decide_eq_true h)) (Pos.Raw.lt_next s _)
     if p (s.get i) then
       let i' := s.next i
       splitAux s p i' i' (s.extract b i :: r)
@@ -2911,7 +2998,7 @@ decreasing_by
     rename_i h _ _
     left; exact Nat.sub_lt_sub_left
       (Nat.lt_of_le_of_lt (Nat.sub_le ..) (Nat.gt_of_not_le (mt decide_eq_true h)))
-      (Nat.lt_of_le_of_lt (Nat.sub_le ..) (lt_next s _))
+      (Nat.lt_of_le_of_lt (Nat.sub_le ..) (Pos.Raw.lt_next s _))
   focus
     rename_i i₀ j₀ _ eq h'
     rw [show (sep.next j₀).byteDistance (s.next i₀) = j₀.byteDistance i₀ by
@@ -2919,12 +3006,12 @@ decreasing_by
       rw [(beq_iff_eq ..).1 eq, Nat.add_sub_add_right]; rfl]
     right; exact Nat.sub_lt_sub_left
       (Nat.lt_of_le_of_lt (Nat.le_add_right ..) (Nat.gt_of_not_le (mt decide_eq_true h')))
-      (lt_next sep _)
+      (Pos.Raw.lt_next sep _)
   focus
     rename_i h _
     left; exact Nat.sub_lt_sub_left
       (Nat.lt_of_le_of_lt (Nat.sub_le ..) (Nat.gt_of_not_le (mt decide_eq_true h)))
-      (lt_next s _)
+      (Pos.Raw.lt_next s _)
 
 /--
 Splits a string `s` on occurrences of the separator string `sep`. The default separator is `" "`.
@@ -3195,6 +3282,7 @@ of the string.
 def prevn : Iterator → Nat → Iterator
   | it, 0   => it
   | it, i+1 => prevn it.prev i
+
 end Iterator
 
 def offsetOfPosAux (s : String) (pos : Pos.Raw) (i : Pos.Raw) (offset : Nat) : Nat :=
@@ -3202,7 +3290,7 @@ def offsetOfPosAux (s : String) (pos : Pos.Raw) (i : Pos.Raw) (offset : Nat) : N
   else if h : s.atEnd i then
     offset
   else
-    have := Nat.sub_lt_sub_left (Nat.gt_of_not_le (mt decide_eq_true h)) (lt_next s _)
+    have := Nat.sub_lt_sub_left (Nat.gt_of_not_le (mt decide_eq_true h)) (Pos.Raw.lt_next s _)
     offsetOfPosAux s pos (s.next i) (offset+1)
 termination_by s.endPos.1 - i.1
 
@@ -3231,7 +3319,7 @@ def Internal.offsetOfPosImpl (s : String) (pos : Pos.Raw) : Nat :=
 
 @[specialize] def foldlAux {α : Type u} (f : α → Char → α) (s : String) (stopPos : Pos.Raw) (i : Pos.Raw) (a : α) : α :=
   if h : i < stopPos then
-    have := Nat.sub_lt_sub_left h (lt_next s i)
+    have := Nat.sub_lt_sub_left h (Pos.Raw.lt_next s i)
     foldlAux f s stopPos (s.next i) (f a (s.get i))
   else a
 termination_by stopPos.1 - i.1
@@ -3254,7 +3342,7 @@ def Internal.foldlImpl (f : String → Char → String) (init : String) (s : Str
 
 @[specialize] def foldrAux {α : Type u} (f : Char → α → α) (a : α) (s : String) (i begPos : Pos.Raw) : α :=
   if h : begPos < i then
-    have := String.prev_lt_of_pos s i <| mt (congrArg String.Pos.Raw.byteIdx) <|
+    have := Pos.Raw.prev_lt_of_pos s i <| mt (congrArg String.Pos.Raw.byteIdx) <|
       Ne.symm <| Nat.ne_of_lt <| Nat.lt_of_le_of_lt (Nat.zero_le _) h
     let i := s.prev i
     let a := f (s.get i) a
@@ -3278,7 +3366,7 @@ Examples:
   if h : i < stopPos then
     if p (s.get i) then true
     else
-      have := Nat.sub_lt_sub_left h (lt_next s i)
+      have := Nat.sub_lt_sub_left h (Pos.Raw.lt_next s i)
       anyAux s stopPos p (s.next i)
   else false
 termination_by stopPos.1 - i.1
@@ -3329,7 +3417,7 @@ Examples:
 def Internal.containsImpl (s : String) (c : Char) : Bool :=
   String.contains s c
 
-theorem utf8SetAux_of_gt (c' : Char) : ∀ (cs : List Char) {i p : Pos.Raw}, i > p → utf8SetAux c' cs i p = cs
+theorem Pos.Raw.utf8SetAux_of_gt (c' : Char) : ∀ (cs : List Char) {i p : Pos.Raw}, i > p → utf8SetAux c' cs i p = cs
   | [],    _, _, _ => rfl
   | c::cs, i, p, h => by
     rw [utf8SetAux, if_neg (mt (congrArg (·.1)) (Ne.symm <| Nat.ne_of_lt h)), utf8SetAux_of_gt c' cs]
@@ -3341,13 +3429,13 @@ theorem set_next_add (s : String) (i : Pos.Raw) (c : Char) (b₁ b₂)
   simp [next, get, set, endPos, ← utf8ByteSize'_eq, utf8ByteSize'] at h ⊢
   rw [Nat.add_comm i.1, Nat.add_assoc] at h ⊢
   let rec foo : ∀ cs a b₁ b₂,
-    (utf8GetAux cs a i).utf8Size + b₁ = utf8ByteSize'.go cs + b₂ →
-    (utf8GetAux (utf8SetAux c cs a i) a i).utf8Size + b₁ = utf8ByteSize'.go (utf8SetAux c cs a i) + b₂
+    (Pos.Raw.utf8GetAux cs a i).utf8Size + b₁ = utf8ByteSize'.go cs + b₂ →
+    (Pos.Raw.utf8GetAux (Pos.Raw.utf8SetAux c cs a i) a i).utf8Size + b₁ = utf8ByteSize'.go (Pos.Raw.utf8SetAux c cs a i) + b₂
   | [], _, _, _, h => h
   | c'::cs, a, b₁, b₂, h => by
-    unfold utf8SetAux
-    apply iteInduction (motive := fun p => (utf8GetAux p a i).utf8Size + b₁ = utf8ByteSize'.go p + b₂) <;>
-      intro h' <;> simp [utf8GetAux, h', utf8ByteSize'.go] at h ⊢
+    unfold Pos.Raw.utf8SetAux
+    apply iteInduction (motive := fun p => (Pos.Raw.utf8GetAux p a i).utf8Size + b₁ = utf8ByteSize'.go p + b₂) <;>
+      intro h' <;> simp [Pos.Raw.utf8GetAux, h', utf8ByteSize'.go] at h ⊢
     next =>
       rw [Nat.add_assoc, Nat.add_left_comm] at h ⊢; rw [Nat.add_left_cancel h]
     next =>
@@ -3359,7 +3447,7 @@ theorem mapAux_lemma (s : String) (i : Pos.Raw) (c : Char) (h : ¬s.atEnd i) :
     (s.set i c).endPos.1 - ((s.set i c).next i).1 < s.endPos.1 - i.1 := by
   suffices (s.set i c).endPos.1 - ((s.set i c).next i).1 = s.endPos.1 - (s.next i).1 by
     rw [this]
-    apply Nat.sub_lt_sub_left (Nat.gt_of_not_le (mt decide_eq_true h)) (lt_next ..)
+    apply Nat.sub_lt_sub_left (Nat.gt_of_not_le (mt decide_eq_true h)) (Pos.Raw.lt_next ..)
   have := set_next_add s i c (s.endPos.byteIdx - (s.next i).byteIdx) 0
   have := set_next_add s i c 0 ((s.next i).byteIdx - s.endPos.byteIdx)
   omega
@@ -3436,8 +3524,11 @@ def toNat? (s : String) : Option Nat :=
 Checks whether substrings of two strings are equal. Substrings are indicated by their starting
 positions and a size in _UTF-8 bytes_. Returns `false` if the indicated substring does not exist in
 either string.
+
+This is a legacy function. The recommended alternative is to construct slices representing the
+strings to be compared and use the `BEq` instance of `String.Slice`.
 -/
-def substrEq (s1 : String) (pos1 : String.Pos.Raw) (s2 : String) (pos2 : String.Pos.Raw) (sz : Nat) : Bool :=
+def Pos.Raw.substrEq (s1 : String) (pos1 : String.Pos.Raw) (s2 : String) (pos2 : String.Pos.Raw) (sz : Nat) : Bool :=
   pos1.byteIdx + sz ≤ s1.endPos.byteIdx && pos2.byteIdx + sz ≤ s2.endPos.byteIdx && loop pos1 pos2 { byteIdx := pos1.byteIdx + sz }
 where
   loop (off1 off2 stop1 : Pos.Raw) :=
@@ -3451,6 +3542,10 @@ where
     have := Nat.sub_lt_sub_left _h (Nat.add_lt_add_left c₁.utf8Size_pos off1.1)
     decreasing_tactic
 
+@[deprecated Pos.Raw.substrEq (since := "2025-10-10")]
+def substrEq (s1 : String) (pos1 : String.Pos.Raw) (s2 : String) (pos2 : String.Pos.Raw) (sz : Nat) : Bool :=
+  Pos.Raw.substrEq s1 pos1 s2 pos2 sz
+
 /--
 Checks whether the first string (`p`) is a prefix of the second (`s`).
 
@@ -3462,7 +3557,7 @@ Examples:
  * `"".isPrefixOf "red green blue" = true`
 -/
 def isPrefixOf (p : String) (s : String) : Bool :=
-  substrEq p 0 s 0 p.endPos.byteIdx
+  Pos.Raw.substrEq p 0 s 0 p.endPos.byteIdx
 
 @[export lean_string_isprefixof]
 def Internal.isPrefixOfImpl (p : String) (s : String) : Bool :=
@@ -3485,11 +3580,11 @@ def replace (s pattern replacement : String) : String :=
         acc ++ s.extract accStop s.endPos
       else
         have := Nat.lt_of_lt_of_le (Nat.add_lt_add_left hPatt _) (Nat.ge_of_not_lt h)
-        if s.substrEq pos pattern 0 pattern.endPos.byteIdx then
+        if Pos.Raw.substrEq s pos pattern 0 pattern.endPos.byteIdx then
           have := Nat.sub_lt_sub_left this (Nat.add_lt_add_left hPatt _)
           loop (acc ++ s.extract accStop pos ++ replacement) (pos + pattern) (pos + pattern)
         else
-          have := Nat.sub_lt_sub_left this (lt_next s pos)
+          have := Nat.sub_lt_sub_left this (Pos.Raw.lt_next s pos)
           loop acc accStop (s.next pos)
       termination_by s.endPos.1 - pos.1
     loop "" 0 0
@@ -3573,7 +3668,7 @@ theorem lt_next (s : Substring) (i : String.Pos.Raw) (h : i.1 < s.bsize) :
     refine mt (congrArg String.Pos.Raw.byteIdx) (Nat.ne_of_lt ?_)
     exact (Nat.add_comm .. ▸ Nat.add_lt_of_lt_sub h :)
   apply Nat.lt_sub_of_add_lt
-  rw [Nat.add_comm]; apply String.lt_next
+  rw [Nat.add_comm]; apply String.Pos.Raw.lt_next
 
 /--
 Returns the previous position in a substring, just prior to the given position. If the position is
@@ -3780,7 +3875,7 @@ Checks whether a substring contains the specified character.
 @[specialize] def takeWhileAux (s : String) (stopPos : String.Pos.Raw) (p : Char → Bool) (i : String.Pos.Raw) : String.Pos.Raw :=
   if h : i < stopPos then
     if p (s.get i) then
-      have := Nat.sub_lt_sub_left h (String.lt_next s i)
+      have := Nat.sub_lt_sub_left h (String.Pos.Raw.lt_next s i)
       takeWhileAux s stopPos p (s.next i)
     else i
   else i
@@ -3812,7 +3907,7 @@ the predicate always returns `true`.
 
 @[specialize] def takeRightWhileAux (s : String) (begPos : String.Pos.Raw) (p : Char → Bool) (i : String.Pos.Raw) : String.Pos.Raw :=
   if h : begPos < i then
-    have := String.prev_lt_of_pos s i <| mt (congrArg String.Pos.Raw.byteIdx) <|
+    have := String.Pos.Raw.prev_lt_of_pos s i <| mt (congrArg String.Pos.Raw.byteIdx) <|
       Ne.symm <| Nat.ne_of_lt <| Nat.lt_of_le_of_lt (Nat.zero_le _) h
     let i' := s.prev i
     let c  := s.get i'
@@ -3924,7 +4019,7 @@ instead, they are equal if they contain the same sequence of characters.
 def beq (ss1 ss2 : Substring) : Bool :=
   let ss1 := ss1.repair
   let ss2 := ss2.repair
-  ss1.bsize == ss2.bsize && ss1.str.substrEq ss1.startPos ss2.str ss2.startPos ss1.bsize
+  ss1.bsize == ss2.bsize && String.Pos.Raw.substrEq ss1.str ss1.startPos ss2.str ss2.startPos ss1.bsize
 
 @[export lean_substring_beq]
 def Internal.beqImpl (ss1 ss2 : Substring) : Bool :=
@@ -3952,7 +4047,7 @@ where
   loop spos tpos :=
     if h : spos < s.stopPos ∧ tpos < t.stopPos then
       if s.str.get spos == t.str.get tpos then
-        have := Nat.sub_lt_sub_left h.1 (s.str.lt_next spos)
+        have := Nat.sub_lt_sub_left h.1 (String.Pos.Raw.lt_next s.str spos)
         loop (s.str.next spos) (t.str.next tpos)
       else
         spos
@@ -3974,7 +4069,7 @@ where
       let spos' := s.str.prev spos
       let tpos' := t.str.prev tpos
       if s.str.get spos' == t.str.get tpos' then
-        have : spos' < spos := s.str.prev_lt_of_pos spos (String.Pos.Raw.ne_zero_of_lt h.1)
+        have : spos' < spos := String.Pos.Raw.prev_lt_of_pos s.str spos (String.Pos.Raw.ne_zero_of_lt h.1)
         loop spos' tpos'
       else
         spos
@@ -4213,12 +4308,16 @@ Examples:
 * `let s := "a  "; s.get (s.nextWhile Char.isWhitespace 0) = 'a'`
 * `let s := "ba  "; s.get (s.nextWhile Char.isWhitespace 0) = 'b'`
 -/
-@[inline] def nextWhile (s : String) (p : Char → Bool) (i : String.Pos.Raw) : String.Pos.Raw :=
+@[inline] def Pos.Raw.nextWhile (s : String) (p : Char → Bool) (i : String.Pos.Raw) : String.Pos.Raw :=
   Substring.takeWhileAux s s.endPos p i
+
+@[deprecated Pos.Raw.nextWhile (since := "2025-10-10")]
+abbrev nextWhile (s : String) (p : Char → Bool) (i : String.Pos.Raw) : String.Pos.Raw :=
+  Pos.Raw.nextWhile s p i
 
 @[export lean_string_nextwhile]
 def Internal.nextWhileImpl (s : String) (p : Char → Bool) (i : String.Pos.Raw) : String.Pos.Raw :=
-  String.nextWhile s p i
+  i.nextWhile s p
 
 /--
 Repeatedly increments a position in a string, as if by `String.next`, while the predicate `p`
@@ -4230,8 +4329,12 @@ Examples:
 * `let s := "   a  "; s.get (s.nextUntil Char.isLetter 0) = 'a'`
 * `let s := "a  "; s.get (s.nextUntil Char.isWhitespace 0) = ' '`
 -/
-@[inline] def nextUntil (s : String) (p : Char → Bool) (i : String.Pos.Raw) : String.Pos.Raw :=
+@[inline] def Pos.Raw.nextUntil (s : String) (p : Char → Bool) (i : String.Pos.Raw) : String.Pos.Raw :=
   nextWhile s (fun c => !p c) i
+
+@[deprecated Pos.Raw.nextUntil (since := "2025-10-10")]
+def nextUntil (s : String) (p : Char → Bool) (i : String.Pos.Raw) : String.Pos.Raw :=
+  i.nextUntil s p
 
 /--
 Replaces each character in `s` with the result of applying `Char.toUpper` to it.
@@ -4416,38 +4519,65 @@ theorem add_eq {p₁ p₂ : Pos.Raw} : p₂.offsetBy p₁ = ⟨p₁.byteIdx + p�
 @[deprecated byteIdx_unoffsetBy (since := "2025-10-08")]
 theorem sub_byteIdx (p₁ p₂ : Pos.Raw) : (p₁.unoffsetBy p₂).byteIdx = p₁.byteIdx - p₂.byteIdx := rfl
 
-@[simp] theorem addChar_byteIdx (p : Pos.Raw) (c : Char) : (p + c).byteIdx = p.byteIdx + c.utf8Size := rfl
+@[deprecated byteIdx_add_char (since := "2025-10-10")]
+theorem addChar_byteIdx (p : Pos.Raw) (c : Char) : (p + c).byteIdx = p.byteIdx + c.utf8Size :=
+  byteIdx_add_char
 
-theorem addChar_eq (p : Pos.Raw) (c : Char) : p + c = ⟨p.byteIdx + c.utf8Size⟩ := rfl
+theorem add_char_eq (p : Pos.Raw) (c : Char) : p + c = ⟨p.byteIdx + c.utf8Size⟩ := rfl
 
-theorem zero_addChar_byteIdx (c : Char) : ((0 : Pos.Raw) + c).byteIdx = c.utf8Size := by
-  simp only [addChar_byteIdx, byteIdx_zero, Nat.zero_add]
+@[deprecated add_char_eq (since := "2025-10-10")]
+theorem addChar_eq (p : Pos.Raw) (c : Char) : p + c = ⟨p.byteIdx + c.utf8Size⟩ :=
+  add_char_eq p c
 
-theorem zero_addChar_eq (c : Char) : (0 : Pos.Raw) + c = ⟨c.utf8Size⟩ := by rw [← zero_addChar_byteIdx]
+theorem byteIdx_zero_add_char (c : Char) : ((0 : Pos.Raw) + c).byteIdx = c.utf8Size := by
+  simp only [byteIdx_add_char, byteIdx_zero, Nat.zero_add]
 
-theorem addChar_right_comm (p : Pos.Raw) (c₁ c₂ : Char) : p + c₁ + c₂ = p + c₂ + c₁ := by
+@[deprecated byteIdx_zero_add_char (since := "2025-10-10")]
+theorem zero_addChar_byteIdx (c : Char) : ((0 : Pos.Raw) + c).byteIdx = c.utf8Size :=
+  byteIdx_zero_add_char c
+
+theorem zero_add_char_eq (c : Char) : (0 : Pos.Raw) + c = ⟨c.utf8Size⟩ := by rw [← byteIdx_zero_add_char]
+
+@[deprecated zero_add_char_eq (since := "2025-10-10")]
+theorem zero_addChar_eq (c : Char) : (0 : Pos.Raw) + c = ⟨c.utf8Size⟩ :=
+  zero_add_char_eq c
+
+theorem add_char_right_comm (p : Pos.Raw) (c₁ c₂ : Char) : p + c₁ + c₂ = p + c₂ + c₁ := by
   apply Pos.Raw.ext
-  repeat rw [pos_add_char]
+  repeat rw [Pos.Raw.pos_add_char]
   apply Nat.add_right_comm
+
+@[deprecated add_char_right_comm (since := "2025-10-10")]
+theorem addChar_right_comm (p : Pos.Raw) (c₁ c₂ : Char) : p + c₁ + c₂ = p + c₂ + c₁ :=
+  add_char_right_comm p c₁ c₂
 
 theorem ne_of_gt {i₁ i₂ : Pos.Raw} (h : i₁ < i₂) : i₂ ≠ i₁ := (ne_of_lt h).symm
 
-@[simp] theorem byteIdx_addString (p : Pos.Raw) (s : String) :
-    (p + s).byteIdx = p.byteIdx + s.utf8ByteSize := rfl
+@[deprecated byteIdx_add_string (since := "2025-10-10")]
+theorem byteIdx_addString (p : Pos.Raw) (s : String) :
+    (p + s).byteIdx = p.byteIdx + s.utf8ByteSize := byteIdx_add_string
 
 @[deprecated byteIdx_addString (since := "2025-03-18")]
-abbrev addString_byteIdx := @byteIdx_addString
+abbrev addString_byteIdx := @byteIdx_add_string
 
 theorem addString_eq (p : Pos.Raw) (s : String) : p + s = ⟨p.byteIdx + s.utf8ByteSize⟩ := rfl
 
-theorem byteIdx_zero_addString (s : String) : ((0 : Pos.Raw) + s).byteIdx = s.utf8ByteSize := by
-  simp only [byteIdx_addString, byteIdx_zero, Nat.zero_add]
+theorem byteIdx_zero_add_string (s : String) : ((0 : Pos.Raw) + s).byteIdx = s.utf8ByteSize := by
+  simp only [byteIdx_add_string, byteIdx_zero, Nat.zero_add]
+
+@[deprecated byteIdx_zero_add_string (since := "2025-10-10")]
+theorem byteIdx_zero_addString (s : String) : ((0 : Pos.Raw) + s).byteIdx = s.utf8ByteSize :=
+  byteIdx_zero_add_string s
 
 @[deprecated byteIdx_zero_addString (since := "2025-03-18")]
-abbrev zero_addString_byteIdx := @byteIdx_zero_addString
+abbrev zero_addString_byteIdx := @byteIdx_zero_add_string
 
-theorem zero_addString_eq (s : String) : (0 : Pos.Raw) + s = ⟨s.utf8ByteSize⟩ := by
-  rw [← byteIdx_zero_addString]
+theorem zero_add_string_eq (s : String) : (0 : Pos.Raw) + s = ⟨s.utf8ByteSize⟩ := by
+  rw [← byteIdx_zero_add_string]
+
+@[deprecated zero_add_string_eq (since := "2025-10-10")]
+theorem zero_addString_eq (s : String) : (0 : Pos.Raw) + s = ⟨s.utf8ByteSize⟩ :=
+  zero_add_string_eq s
 
 @[simp] theorem mk_le_mk {i₁ i₂ : Nat} : Pos.Raw.mk i₁ ≤ Pos.Raw.mk i₂ ↔ i₁ ≤ i₂ := .rfl
 
@@ -4457,11 +4587,17 @@ end Pos.Raw
 
 @[simp] theorem get!_eq_get (s : String) (p : Pos.Raw) : get! s p = get s p := rfl
 
-theorem lt_next' (s : String) (p : Pos.Raw) : p < next s p := lt_next ..
+@[deprecated Pos.Raw.lt_next (since := "2025-10-10")]
+theorem lt_next' (s : String) (p : Pos.Raw) : p < next s p :=
+  Pos.Raw.lt_next s p
 
-@[simp] theorem prev_zero (s : String) : prev s 0 = 0 := by
-  rw [prev]
+@[simp] theorem Pos.Raw.prev_zero (s : String) : Pos.Raw.prev s 0 = 0 := by
+  rw [Pos.Raw.prev]
   cases s.data <;> simp [utf8PrevAux, Pos.Raw.le_iff]
+
+@[deprecated Pos.Raw.prev_zero (since := "2025-10-10")]
+theorem prev_zero (s : String) : prev s 0 = 0 := by
+  exact Pos.Raw.prev_zero s
 
 @[simp] theorem get'_eq (s : String) (p : Pos.Raw) (h) : get' s p h = get s p := rfl
 
